Use BufferView for buffer64 in Memory_i_s + most of the proofs

src/arch/x64/X64.Memory_i_s.fst
@@ -1,9 +1,10 @@
 module X64.Memory_i_s
 
-module I = Interop64
+module I = Interop
 module HS = FStar.HyperStack
 module B = LowStar.Buffer
 module M = LowStar.Modifies
+module BV = LowStar.BufferView
 module S = X64.Bytes_Semantics_s
 module H = FStar.Heap
 
@@ -12,11 +13,11 @@ module H = FStar.Heap
 let heap = H.heap
 noeq type mem' = {
   addrs : I.addr_map;
-  ptrs : list (B.buffer UInt64.t);
+  ptrs : list (B.buffer UInt8.t);
   hs : HS.mem;
   }
 
-type mem = (m:mem'{I.list_disjoint_or_eq #UInt64.t m.ptrs /\
+type mem = (m:mem'{I.list_disjoint_or_eq #UInt8.t m.ptrs /\
   I.list_live m.hs m.ptrs})
 
 let op_String_Access = Map.sel
@@ -38,7 +39,7 @@ let m_of_typ (t:typ) : Type0 =
   | TBase TUInt16 -> tuint16
   | TBase TUInt32 -> tuint32
   | TBase TUInt64 -> tuint64
-  | TBase TUInt128 -> admit () // M.tuint128
+  | TBase TUInt128 -> quad32
 
 let v_of_typ (t:typ) (v:type_of_typ t) :  (m_of_typ t) =
   match t with
@@ -67,17 +68,34 @@ let lemma_v_to_of_typ (t:typ) (v:type_of_typ t) : Lemma
   | TBase TUInt64 -> assert (UInt64.v (UInt64.uint_to_t v) == v)
   | TBase TUInt128 -> admit()
 
-let buffer t = B.buffer (m_of_typ t)
+let view_n = function
+  | TBase TUInt8 -> 1
+  | TBase TUInt16 -> 2
+  | TBase TUInt32 -> 4
+  | TBase TUInt64 -> 8
+  | TBase TUInt128 -> 16
+
+assume val uint64_view: (v:BV.view UInt8.t UInt64.t{BV.View?.n v == view_n (TBase TUInt64)})
+assume val uint128_view: (v:BV.view UInt8.t quad32{BV.View?.n v == view_n (TBase TUInt128)})
+
+val uint_view (t:typ) : (v:BV.view UInt8.t (m_of_typ t){BV.View?.n v == view_n t})
+
+let uint_view = function
+  | TBase TUInt64 -> uint64_view
+  | TBase TUInt128 -> uint128_view
+  | _ -> admit()
+
+let buffer t = (b:B.buffer UInt8.t{B.length b % view_n t == 0})
 
 let buffer_as_seq #t h b =
-  let s = B.as_seq h.hs b in
+  let s = BV.as_seq h.hs (BV.mk_buffer_view b (uint_view t)) in
   let len = Seq.length s in
   let contents (i:nat{i < len}) : type_of_typ t = v_to_typ t (Seq.index s i) in
   Seq.init len contents
 
 // TODO: Fix this
-let buffer_readable #t h b = if (t = TBase TUInt64) then List.memP b h.ptrs else false
-let buffer_length #t b = B.length b
+let buffer_readable #t h b = List.memP b h.ptrs
+let buffer_length #t b = BV.length (BV.mk_buffer_view b (uint_view t))
 let loc = M.loc
 let loc_none = M.loc_none
 let loc_union = M.loc_union
@@ -88,17 +106,17 @@ let modifies s h h' =
   let _ = () in
   M.modifies s h.hs h'.hs /\ h.ptrs == h'.ptrs /\ h.addrs == h'.addrs
 
-let valid_state s = s.state.S.mem == I.down_mem64 s.mem.hs s.mem.addrs s.mem.ptrs
+let valid_state s = s.state.S.mem == I.down_mem s.mem.hs s.mem.addrs s.mem.ptrs
 
 let frame_valid s = ()
 
-let get_heap h = I.down_mem64 h.hs h.addrs h.ptrs
+let get_heap h = I.down_mem h.hs h.addrs h.ptrs
 
 let same_heap s1 s2 = ()
 
 let buffer_addr #t b h =
   let addrs = h.addrs in
-  addrs (m_of_typ t) b
+  addrs b
 
 let loc_readable h s = unit // admit()
 let loc_readable_none = admit()
@@ -128,6 +146,10 @@ let modifies_buffer_elim #t1 b p h h' =
   if buffer_length b > 0 then
   (
     M.modifies_buffer_elim b p h.hs h'.hs;
+    assert (Seq.equal (B.as_seq h.hs b) (B.as_seq h'.hs b));
+    //TODO: Need an additional lemma about buffer views here relating underlying seq and view seq
+    // Could perhaps be proven recursively using get/put_sel
+    admit();
     assert (Seq.equal (buffer_as_seq h b) (buffer_as_seq h' b));
     ()
   )
@@ -172,21 +194,54 @@ let buffer_read #t b i h =
   if i < 0 || i >= buffer_length b then default_of_typ t else
   Seq.index (buffer_as_seq h b) i
 
+val seq_upd (#b:_)
+            (h:HS.mem)
+            (vb:BV.buffer b{BV.live h vb})
+            (i:nat{i < BV.length vb})
+            (x:b)
+  : Lemma (Seq.equal
+      (Seq.upd (BV.as_seq h vb) i x)
+      (BV.as_seq (BV.upd h vb i x) vb))
+
+let seq_upd #b h vb i x =
+  let old_s = BV.as_seq h vb in
+  let new_s = BV.as_seq (BV.upd h vb i x) vb in
+  let upd_s = Seq.upd old_s i x in
+  let rec aux (k:nat) : Lemma 
+    (requires (k <= Seq.length upd_s /\ (forall (j:nat). j < k ==> Seq.index upd_s j == Seq.index new_s j)))
+    (ensures (forall (j:nat). j < Seq.length upd_s ==> Seq.index upd_s j == Seq.index new_s j))
+    (decreases %[(Seq.length upd_s) - k]) =
+    if k = Seq.length upd_s then ()
+    else begin
+      BV.sel_upd vb i k x h;
+      BV.as_seq_sel h vb k;
+      BV.as_seq_sel (BV.upd h vb i x) vb k;
+      aux (k+1)
+    end
+  in aux 0;
+  ()
+
 let buffer_write #t b i v h =
  if i < 0 || i >= buffer_length b then h else
- let hs' = B.g_upd_seq b (Seq.upd (B.as_seq h.hs b) i (v_of_typ t v)) h.hs in
- B.g_upd_seq_as_seq b (Seq.upd (B.as_seq h.hs b) i (v_of_typ t v)) h.hs;
- let h':mem = {h with hs = hs'} in
- assert (Seq.equal (buffer_as_seq h' b) (Seq.upd (buffer_as_seq h b) i v));
- h'
+ begin
+   let view = uint_view t in
+   let bv = BV.mk_buffer_view b view in
+   BV.as_buffer_mk_buffer_view b view;
+   BV.upd_modifies h.hs bv i (v_of_typ t v);
+   let hs' = BV.upd h.hs bv i (v_of_typ t v) in
+   let h':mem = {h with hs = hs'} in
+   seq_upd h.hs bv i (v_of_typ t v);
+   assert (Seq.equal (buffer_as_seq h' b) (Seq.upd (buffer_as_seq h b) i v));
+   h'
+ end
 
-val addr_in_ptr: (addr:int) -> (ptr:buffer64) -> (h:mem) ->
-  GTot (b:bool{ not b <==> (forall i. 0 <= i /\ i < B.length ptr ==> 
+val addr_in_ptr64: (addr:int) -> (ptr:buffer64) -> (h:mem) ->
+  GTot (b:bool{ not b <==> (forall i. 0 <= i /\ i < buffer_length ptr ==> 
     addr <> (buffer_addr ptr h) + 8 `op_Multiply` i)})
   
 // Checks if address addr corresponds to one of the elements of buffer ptr
-let addr_in_ptr (addr:int) (ptr:buffer64) (h:mem) =
-  let n = B.length ptr in
+let addr_in_ptr64 (addr:int) (ptr:buffer64) (h:mem) =
+  let n = buffer_length ptr in
   let base = buffer_addr ptr h in
   let rec aux (i:nat) : Tot (b:bool{not b <==> (forall j. i <= j /\ j < n ==> 
     addr <> base + 8 `op_Multiply` j)}) 
@@ -196,57 +251,56 @@ let addr_in_ptr (addr:int) (ptr:buffer64) (h:mem) =
     else aux (i+1)
   in aux 0
 
-let rec get_addr_in_ptr (n base addr:nat) (i:nat{exists j. i <= j /\ j < n /\ base + 8 `op_Multiply` j == addr}) : 
+let rec get_addr_in_ptr64 (n base addr:nat) (i:nat{exists j. i <= j /\ j < n /\ base + 8 `op_Multiply` j == addr}) : 
     GTot (j:nat{base + 8 `op_Multiply` j == addr})
     (decreases %[n-i]) =
     if base + 8 `op_Multiply` i = addr then i
     else if i >= n then i
-    else get_addr_in_ptr n base addr (i+1)
+    else get_addr_in_ptr64 n base addr (i+1)
 
+let valid_buffer64 (addr:int) (b:B.buffer UInt8.t) (h:mem) : GTot bool = B.length b % (view_n (TBase TUInt64)) = 0 && (addr_in_ptr64 addr b h)
 
-let rec valid_mem_aux addr ps (h:mem) : GTot (b:bool{
-  (not b) <==> (forall (x:buffer64). (List.memP x ps ==> not (addr_in_ptr addr x h) ))}) 
+let rec valid_mem_aux64 addr (ps:list (B.buffer UInt8.t)) (h:mem) : GTot (b:bool{
+  (not b) <==> (forall (x:buffer64). (List.memP x ps ==> not (valid_buffer64 addr x h) ))}) 
   = match ps with
     | [] -> false
-    | a::q -> if (addr_in_ptr addr a h) then true else valid_mem_aux addr q h
+    | a::q -> if valid_buffer64 addr a h then true else valid_mem_aux64 addr q h
 
-let valid_mem64 ptr h = valid_mem_aux ptr h.ptrs h
+let valid_mem64 ptr h = valid_mem_aux64 ptr h.ptrs h
 
-let rec load_mem_aux addr (ps:list buffer64) (h:mem{forall x. List.memP x ps ==> List.memP x h.ptrs }) : 
+let rec load_mem_aux64 addr (ps:list (B.buffer UInt8.t)) (h:mem{forall x. List.memP x ps ==> List.memP x h.ptrs }) : 
   GTot nat64 =
   match ps with
   | [] -> 0
   | a::q ->
-    let base = buffer_addr a h in
-    let n = B.length a in
-    if addr_in_ptr addr a h then
+    if valid_buffer64 addr a h then
     begin
-      buffer_read a (get_addr_in_ptr n base addr 0) h
+      let a:buffer64 = a in
+      let base = buffer_addr a h in
+      buffer_read a (get_addr_in_ptr64 (buffer_length a) base addr 0) h
     end
-    else load_mem_aux addr q h
+    else load_mem_aux64 addr q h
 
 let load_mem64 ptr h =
   if not (valid_mem64 ptr h) then 0
-  else load_mem_aux ptr h.ptrs h
+  else load_mem_aux64 ptr h.ptrs h
 
-let rec store_mem_aux addr (ps:list buffer64) (v:nat64) (h:mem{forall x. List.memP x ps ==> List.memP x h.ptrs }) : 
+let rec store_mem_aux64 addr (ps:list (B.buffer UInt8.t)) (v:nat64) (h:mem{forall x. List.memP x ps ==> List.memP x h.ptrs }) : 
   GTot (h1:mem{h.addrs == h1.addrs /\ h.ptrs == h1.ptrs }) =
   match ps with
   | [] -> h
   | a::q ->
-    let base = buffer_addr a h in
-    let n = B.length a in
-    if addr_in_ptr addr a h then
+    if valid_buffer64 addr a h then
     begin
-      buffer_write a (get_addr_in_ptr n base addr 0) v h
+      let a:buffer64 = a in
+      let base = buffer_addr a h in
+      buffer_write a (get_addr_in_ptr64 (buffer_length a) base addr 0) v h
     end
-    else store_mem_aux addr q v h
+    else store_mem_aux64 addr q v h
 
 let store_mem64 i v h =
   if not (valid_mem64 i h) then h
-  else
-  let h1 = store_mem_aux i h.ptrs v h in
-  h1
+  else store_mem_aux64 i h.ptrs v h
 
 let valid_mem128 ptr h = admit()
 let load_mem128 ptr h = admit()
@@ -254,18 +308,29 @@ let store_mem128 ptr v h = admit()
 
 let lemma_valid_mem64 b i h = ()
 
+#set-options "--z3rlimit 20"
+
 let lemma_load_mem64 b i h =
   let addr = buffer_addr b h + 8 `op_Multiply` i in
   lemma_valid_mem64 b i h;
-  let rec aux (ps:list buffer64{I.list_disjoint_or_eq ps})
+  let rec aux (ps:list (B.buffer UInt8.t){I.list_disjoint_or_eq ps})
     (h0:mem{h == h0 /\ (forall x. List.memP x ps ==> List.memP x h0.ptrs)}) :  
-    Lemma (requires (List.memP b ps /\ i < B.length b) )
-    (ensures (load_mem_aux addr ps h0 == buffer_read b i h0)) = 
+    Lemma (requires (List.memP b ps /\ i < buffer_length b) )
+    (ensures (load_mem_aux64 addr ps h0 == buffer_read b i h0)) = 
     match ps with
     | [] -> ()
     | a::q ->
-      if addr_in_ptr addr a h0 then begin
-  	assert (I.disjoint_or_eq a b);
+      if valid_buffer64 addr a h0 then begin
+        let a:buffer64 = a in
+	BV.length_eq (BV.mk_buffer_view a uint64_view);
+	BV.get_view_mk_buffer_view a uint64_view;
+	BV.as_buffer_mk_buffer_view a uint64_view;	
+	BV.length_eq (BV.mk_buffer_view b uint64_view);
+	BV.get_view_mk_buffer_view b uint64_view;
+	BV.as_buffer_mk_buffer_view b uint64_view;
+
+	assert (I.disjoint_or_eq a b);
+	assert (a == b);
   	()
       end
       else begin
@@ -274,21 +339,27 @@ let lemma_load_mem64 b i h =
       end
   in aux h.ptrs h  
 
-#set-options "--z3rlimit 20"
-
 let lemma_store_mem64 b i v h =
   let addr = buffer_addr b h + 8 `op_Multiply` i in
-  let s' = store_mem64 addr v h in
   lemma_valid_mem64 b i h;
-  let rec aux (ps:list buffer64{I.list_disjoint_or_eq ps})
+  let rec aux (ps:list (B.buffer UInt8.t){I.list_disjoint_or_eq ps})
     (h0:mem{h == h0 /\ (forall x. List.memP x ps ==> List.memP x h0.ptrs)}) :  
-    Lemma (requires (List.memP b ps /\ i < B.length b) )
-    (ensures (store_mem_aux addr ps v h0 == buffer_write b i v h0)) = 
+    Lemma (requires (List.memP b ps /\ i < buffer_length b) )
+    (ensures (store_mem_aux64 addr ps v h0 == buffer_write b i v h0)) = 
     match ps with
     | [] -> ()
     | a::q ->
-      if addr_in_ptr addr a h0 then begin
-  	assert (I.disjoint_or_eq a b);
+      if valid_buffer64 addr a h0 then begin
+	let a:buffer64 = a in
+	BV.length_eq (BV.mk_buffer_view a uint64_view);
+	BV.get_view_mk_buffer_view a uint64_view;
+	BV.as_buffer_mk_buffer_view a uint64_view;	
+	BV.length_eq (BV.mk_buffer_view b uint64_view);
+	BV.get_view_mk_buffer_view b uint64_view;
+	BV.as_buffer_mk_buffer_view b uint64_view;
+
+	assert (I.disjoint_or_eq a b);
+	assert (a == b);
   	()
       end
       else begin
@@ -301,11 +372,11 @@ let lemma_valid_mem128 b i h = admit()
 let lemma_load_mem128 b i h = admit()
 let lemma_store_mem128 b i v h = admit()
 
-let rec get_addr_ptr (ptr:int) (h:mem) (ps:list buffer64{valid_mem_aux ptr ps h}) : 
-  GTot (b:buffer64{List.memP b ps /\ addr_in_ptr ptr b h}) =
+let rec get_addr_ptr64 (ptr:int) (h:mem) (ps:list (B.buffer UInt8.t){valid_mem_aux64 ptr ps h}) : 
+  GTot (b:buffer64{List.memP b ps /\ valid_buffer64 ptr b h}) =
   match ps with
   // The list cannot be empty because of the mem predicate
-  | a::q -> if addr_in_ptr ptr a h then a else get_addr_ptr ptr h q
+  | a::q -> if valid_buffer64 ptr a h then a else get_addr_ptr64 ptr h q
 
 let lemma_store_load_mem64 ptr v h = admit()
 let lemma_frame_store_mem64 i v h = admit()
@@ -315,36 +386,105 @@ let lemma_store_load_mem128 ptr v h = admit()
 let lemma_frame_store_mem128 ptr v h = admit()
 let lemma_valid_store_mem128 ptr v h = admit()
 
-#set-options "--z3rlimit 40"
+#set-options "--z3rlimit 100"
 
-let rec written_buffer_down_aux1 (b:buffer64) (i:nat{i < B.length b}) (v:nat64)
-      (ps:list buffer64{I.list_disjoint_or_eq ps /\ List.memP b ps})
+// val same_underlying_sub_seq (#src #dest:Type)
+//                             (h1 h2:HS.mem)
+// 		            (b:B.buffer src)
+// 			    (v:BV.view src dest {
+// 			      B.length b % BV.View?.n v == 0})
+// 			    (i:nat{i < BV.length (BV.mk_buffer_view b v)}):
+//   Lemma 
+//     (requires BV.sel h1 (BV.mk_buffer_view b v) i == BV.sel h2 (BV.mk_buffer_view b v) i)
+//     (ensures Seq.equal (B.as_seq h1 b) (B.as_seq h2 b))
+
+
+// val same_underlying_seq (#src #dest:Type)
+//                         (h1 h2:HS.mem)
+// 		        (b:B.buffer src)
+// 			(v:BV.view src dest {
+// 			  B.length b % BV.View?.n v == 0}) :
+//   Lemma 
+//     (requires Seq.equal 
+//       (BV.as_seq h1 (BV.mk_buffer_view b v))
+//       (BV.as_seq h2 (BV.mk_buffer_view b v)))
+//     (ensures Seq.equal (B.as_seq h1 b) (B.as_seq h2 b))
+
+// let same_underlying_seq #src #dest h1 h2 b v = admit()
+  
+val heap_shift (m1 m2:S.heap) (base:int) (n:nat) : Lemma
+  (requires (forall i. 0 <= i /\ i < n ==> m1.[base + i] == m2.[base + i]))
+  (ensures (forall i. {:pattern (m1.[i])} base <= i /\ i < base + n ==> m1.[i] == m2.[i]))
+	      
+let heap_shift m1 m2 base n =
+  assert (forall i. base <= i /\ i < base + n ==>
+    m1.[base + (i - base)] == m2.[base + (i - base)])
+
+val same_mem_get_heap_val (b:buffer64)
+			  (i:nat{i < buffer_length b})
+			  (v:nat64)
+			  (k:nat{k < buffer_length b})
+			  (h1:mem{List.memP b h1.ptrs})
+			  (h2:mem{h2 == buffer_write b i v h1})
+			  (mem1:S.heap{I.correct_down_p h1.hs h1.addrs mem1 b})
+			  (mem2:S.heap{I.correct_down_p h2.hs h2.addrs mem2 b}) : Lemma
+  (requires (Seq.index (buffer_as_seq h1 b) k == Seq.index (buffer_as_seq h2 b) k))			  
+  (ensures (let ptr = buffer_addr b h1 + 8 `op_Multiply` k in 
+    forall i. i >= 0 /\ i < 8 ==> mem1.[ptr+i] == mem2.[ptr+i]))
+
+let same_mem_get_heap_val b i v k h1 h2 mem1 mem2 =
+  let ptr = buffer_addr b h1 + 8 `op_Multiply` k in
+  let aux (i:nat{i < 8}) : Lemma (mem1.[ptr+i] == mem2.[ptr+i]) =
+    BV.as_seq_sel h1.hs (BV.mk_buffer_view b uint64_view) k;
+    BV.as_seq_sel h2.hs (BV.mk_buffer_view b uint64_view) k;
+    BV.put_sel h1.hs (BV.mk_buffer_view b uint64_view) k;
+    BV.put_sel h2.hs (BV.mk_buffer_view b uint64_view) k;
+    BV.as_buffer_mk_buffer_view b uint64_view;
+    BV.get_view_mk_buffer_view b uint64_view;
+    BV.view_indexing (BV.mk_buffer_view b uint64_view) k;
+    BV.length_eq (BV.mk_buffer_view b uint64_view);
+    let open FStar.Mul in
+    let s1 = (Seq.slice (B.as_seq h1.hs b) (k * 8) (k * 8 + 8)) in
+    let s2 = (Seq.slice (B.as_seq h2.hs b) (k * 8) (k * 8 + 8)) in
+    assert (s1 == s2);
+    assert (Seq.index s1 i == Seq.index (B.as_seq h1.hs b) (k * 8 + i));
+    assert (UInt8.v (Seq.index s1 i) == mem1.[ptr+i]);
+    assert (Seq.index s2 i == Seq.index (B.as_seq h2.hs b) (k * 8 + i));
+    assert (UInt8.v (Seq.index s2 i) == mem2.[ptr+i]);
+    ()
+  in
+  Classical.forall_intro aux;
+  ()
+
+let rec written_buffer_down64_aux1 (b:buffer64) (i:nat{i < buffer_length b}) (v:nat64)
+      (ps:list (B.buffer UInt8.t){I.list_disjoint_or_eq ps /\ List.memP b ps})
       (h:mem{forall x. List.memP x ps ==> List.memP x h.ptrs})
       (base:nat{base == buffer_addr b h})
       (k:nat) (h1:mem{h1 == buffer_write b i v h}) 
-      (mem1:S.heap{I.correct_down64 h.hs h.addrs ps mem1}) 
+      (mem1:S.heap{I.correct_down h.hs h.addrs ps mem1}) 
       (mem2:S.heap{
-      (I.correct_down64 h1.hs h.addrs ps mem2) /\
+      (I.correct_down h1.hs h.addrs ps mem2) /\
       (forall j. base <= j /\ j < base + k `op_Multiply` 8 ==> mem1.[j] == mem2.[j])}) : 
       Lemma (requires True)
       (ensures (forall j. j >= base /\ j < base + 8 `op_Multiply` i ==> mem1.[j] == mem2.[j]))
       (decreases %[i-k]) =
     if k >= i then ()
     else begin
-      assert (Seq.index (buffer_as_seq h1 b) k == Seq.index (buffer_as_seq h b) k);
-      Bytes_Semantics_i.same_mem_get_heap_val (base + 8 `op_Multiply` k) mem1 mem2;
-      written_buffer_down_aux1 b i v ps h base (k+1) h1 mem1 mem2
+      let ptr = base + 8 `op_Multiply` k in
+      same_mem_get_heap_val b i v k h h1 mem1 mem2;
+      heap_shift mem1 mem2 ptr 8;
+      written_buffer_down64_aux1 b i v ps h base (k+1) h1 mem1 mem2
     end
 
-let rec written_buffer_down_aux2 (b:buffer64) (i:nat{i < B.length b}) (v:nat64)
-      (ps:list buffer64{I.list_disjoint_or_eq ps /\ List.memP b ps})
+let rec written_buffer_down64_aux2 (b:buffer64) (i:nat{i < B.length b}) (v:nat64)
+      (ps:list (B.buffer UInt8.t){I.list_disjoint_or_eq ps /\ List.memP b ps})
       (h:mem{forall x. List.memP x ps ==> List.memP x h.ptrs})
       (base:nat{base == buffer_addr b h})
-      (n:nat{n == B.length b})
+      (n:nat{n == buffer_length b})
       (k:nat{k > i}) (h1:mem{h1 == buffer_write b i v h}) 
-      (mem1:S.heap{I.correct_down64 h.hs h.addrs ps mem1}) 
+      (mem1:S.heap{I.correct_down h.hs h.addrs ps mem1}) 
       (mem2:S.heap{
-      (I.correct_down64 h1.hs h.addrs ps mem2) /\
+      (I.correct_down h1.hs h.addrs ps mem2) /\
       (forall j. base + 8 `op_Multiply` (i+1) <= j /\ j < base + k `op_Multiply` 8 ==>
       mem1.[j] == mem2.[j])}) :
       Lemma 
@@ -354,29 +494,30 @@ let rec written_buffer_down_aux2 (b:buffer64) (i:nat{i < B.length b}) (v:nat64)
       (decreases %[n-k]) =
     if k >= n then ()
     else begin
-      assert (Seq.index (buffer_as_seq h1 b) k == Seq.index (buffer_as_seq h b) k);    
-       Bytes_Semantics_i.same_mem_get_heap_val (base + 8 `op_Multiply` k) mem1 mem2;
-      written_buffer_down_aux2 b i v ps h base n (k+1) h1 mem1 mem2
+      let ptr = base + 8 `op_Multiply` k in
+      same_mem_get_heap_val b i v k h h1 mem1 mem2;
+      heap_shift mem1 mem2 ptr 8;
+      written_buffer_down64_aux2 b i v ps h base n (k+1) h1 mem1 mem2
     end
     
-let written_buffer_down (b:buffer64) (i:nat{i < B.length b}) (v:nat64)
-  (ps: list buffer64{I.list_disjoint_or_eq ps /\ List.memP b ps}) (h:mem{forall x. List.memP x ps ==> List.memP x h.ptrs}) :
+let written_buffer_down64 (b:buffer64) (i:nat{i < B.length b}) (v:nat64)
+  (ps: list (B.buffer UInt8.t){I.list_disjoint_or_eq ps /\ List.memP b ps}) (h:mem{forall x. List.memP x ps ==> List.memP x h.ptrs}) :
   Lemma (
-    let mem1 = I.down_mem64 h.hs h.addrs ps in
+    let mem1 = I.down_mem h.hs h.addrs ps in
     let h1 = buffer_write b i v h in
-    let mem2 = I.down_mem64 h1.hs h.addrs ps in
+    let mem2 = I.down_mem h1.hs h.addrs ps in
     let base = buffer_addr b h in
     let n = B.length b in
     forall j. (base <= j /\ j < base + 8 `op_Multiply` i) \/ 
 	 (base + 8 `op_Multiply` (i+1) <= j /\ j < base + 8 `op_Multiply` n) ==>
 	 mem1.[j] == mem2.[j]) = 
-    let mem1 = I.down_mem64 h.hs h.addrs ps in
+    let mem1 = I.down_mem h.hs h.addrs ps in
     let h1 = buffer_write b i v h in
-    let mem2 = I.down_mem64 h1.hs h.addrs ps in	 
+    let mem2 = I.down_mem h1.hs h.addrs ps in	 
     let base = buffer_addr b h in
     let n = B.length b in
-    written_buffer_down_aux1 b i v ps h base 0 h1 mem1 mem2;
-    written_buffer_down_aux2 b i v ps h base n (i+1) h1 mem1 mem2
+    written_buffer_down64_aux1 b i v ps h base 0 h1 mem1 mem2;
+    written_buffer_down64_aux2 b i v ps h base n (i+1) h1 mem1 mem2
 
 #set-options "--z3rlimit 50"
 
